### Original input with jump target labels marked

```
cpy 1 a       a = 1
cpy 1 b       b = 1
cpy 26 d      d = 26
jnz c 2       -> A    not taken
jnz 1 5       -> B    always taken
A: cpy 7 c    c = 7
C: inc d      d += 1
dec c         c -= 1
jnz c -2      -> C
B: cpy a c    c = a
D: inc a      a += 1
dec b         b -= 1
jnz b -2      -> D
cpy c b       b = c
dec d         d -= 1
jnz d -6      -> B
cpy 16 c      c = 16
F: cpy 17 d   d = 17
E: inc a      a += 1
dec d         d -= 1
jnz d -2      -> E
dec c         c -= 1
jnz c -5      -> F
```


### First rewrite

```
a = 1
b = 1
d = 26
if (c != 0) {
    goto A
}
goto B

A:
for (c = 7; c > 0; c--) {
  d++
}

B:
do {
    c = a
    do {
        a++
        b--
    } while (b != 0)

    b = c
    d--
} while (d != 0)

c = 16
F:
do {
    d = 17
    do {
        a++
        d--
    } while (d != 0)
    c--
} while (c != 0)

print(a)
```

### Loops interpreted

```
a = 1
b = 1
d = 26
if (c != 0) {
    // not taken in part 1, taken in part 2
    d += 7
    c = 0
}

for (; d > 0; d--) {
    c = a
    a += b
    b = c
}

a += 16 * 17
```

### Program interpretation
The main loop calculates fibonacci number from the value of `d`, which is 26 in part 1 and 33 in part 2. At the end, the constant 16 * 17 is added to the result.

* fib(26) = 317811
* part1 = 318083
* fib(33) = 9227465
* part2 = 9227737
